ContextLogic/theories/LogicQualifier.v
@@ -21,6 +21,7 @@ Context {V : Type} `{ValueSig V}.
 Local Notation WorldT := (World (V := V)) (only parsing).
 Local Notation WfWorldT := (WfWorld (V := V)) (only parsing).
 Local Notation LStoreT := (gmap logic_var V) (only parsing).
+Local Notation LWorldT := (LWorld (V := V)) (only parsing).
 Local Notation LWorldOnT := (LWorldOn (V := V)) (only parsing).
 
 Record logic_qualifier : Type := lqual {
@@ -106,6 +107,92 @@ Definition lqual_msubst_store
     (σ : Store (V := V)) (q : logic_qualifier) : logic_qualifier :=
   lqual_mlsubst (lstore_lift_free σ) q.
 
+Lemma lworld_on_mlsubst_back_union
+    (D : lvset) (ρ1 ρ2 : LStoreT)
+    (w1 : LWorldOnT ((D ∖ dom (ρ1 : gmap logic_var V))
+      ∖ dom (ρ2 : gmap logic_var V)))
+    (w2 : LWorldOnT (D ∖ dom (ρ1 ∪ ρ2 : gmap logic_var V))) :
+  storeA_compat ρ1 ρ2 ->
+  @lw V _ w1 = @lw V _ w2 ->
+  lworld_on_mlsubst_back D ρ1
+    (lworld_on_mlsubst_back (D ∖ dom (ρ1 : gmap logic_var V)) ρ2 w1) =
+  lworld_on_mlsubst_back D (ρ1 ∪ ρ2) w2.
+Proof.
+  intros Hcompat Hlw.
+  assert (Hwiff : forall σ,
+      (@lw V _ w1 : LWorld) σ <-> (@lw V _ w2 : LWorld) σ).
+  { intros σ. rewrite Hlw. reflexivity. }
+  apply lworld_on_ext.
+  apply wfworldA_ext. apply worldA_ext.
+  - set (wl := lworld_on_mlsubst_back D ρ1
+        (lworld_on_mlsubst_back (D ∖ dom (ρ1 : gmap logic_var V)) ρ2 w1)).
+    set (wr := lworld_on_mlsubst_back D
+        (@union (gmap logic_var V) _ ρ1 ρ2) w2).
+    change (lworld_dom (lraw_world (lw D wl)) =
+      lworld_dom (lraw_world (lw D wr))).
+    rewrite (lw_dom D wl), (lw_dom D wr).
+    reflexivity.
+  - unfold lworld_on_mlsubst_back.
+    intros σ. cbn [lw resA_product rawA_product singleton_worldA worldA_stores
+      proj1_sig].
+    split.
+    + intros (σ12 & σ1 & Hσ12 & -> & Hc12_1 & ->).
+      destruct Hσ12 as (σ0 & σ2' & Hσ0 & -> & Hc0_2 & ->).
+      exists σ0, (storeA_restrict (ρ1 ∪ ρ2) D). repeat split; auto.
+      * apply Hwiff. exact Hσ0.
+      * rewrite <- storeA_restrict_union_residual_l by exact Hcompat.
+        apply storeA_compat_union_intro_r.
+        -- exact Hc0_2.
+        -- eapply storeA_compat_union_inv_l. exact Hc12_1.
+      * rewrite <- map_union_assoc.
+        rewrite storeA_restrict_union_residual_l by exact Hcompat.
+        reflexivity.
+    + intros (σ0 & σ12 & Hσ0 & -> & Hc0_12 & ->).
+      assert (Hc0_12' : storeA_compat σ0
+          (@union (gmap logic_var V) _
+            (storeA_restrict ρ2 (D ∖ dom (ρ1 : gmap logic_var V)))
+            (storeA_restrict ρ1 D))).
+      {
+        rewrite storeA_restrict_union_residual_l by exact Hcompat.
+        exact Hc0_12.
+      }
+      assert (Hc0_res : storeA_compat σ0
+          (storeA_restrict ρ2 (D ∖ dom (ρ1 : gmap logic_var V)))).
+      { eapply storeA_compat_union_r_inv_l. exact Hc0_12'. }
+      assert (Hres_1 : storeA_compat
+          (storeA_restrict ρ2 (D ∖ dom (ρ1 : gmap logic_var V)))
+          (storeA_restrict ρ1 D)).
+      {
+        apply storeA_compat_sym.
+        apply storeA_compat_restrict_r.
+        eapply (storeA_compat_restrict_l_full_r
+          (storeA_restrict ρ1 D) ρ2 D).
+        - rewrite storeA_restrict_dom. better_set_solver.
+        - apply storeA_compat_restrict. exact Hcompat.
+      }
+      assert (Hc0_1 : storeA_compat σ0 (storeA_restrict ρ1 D)).
+      { eapply storeA_compat_union_r_inv_r; [exact Hres_1 | exact Hc0_12']. }
+      exists (@union (gmap logic_var V) _
+          σ0 (storeA_restrict ρ2 (D ∖ dom (ρ1 : gmap logic_var V)))).
+      exists (storeA_restrict ρ1 D).
+      split.
+      * exists σ0, (storeA_restrict ρ2 (D ∖ dom (ρ1 : gmap logic_var V))).
+        split.
+        -- apply (proj2 (Hwiff σ0)). exact Hσ0.
+        -- split.
+           ++ reflexivity.
+           ++ split.
+              ** exact Hc0_res.
+              ** reflexivity.
+      * split.
+        -- reflexivity.
+        -- split.
+           ++ apply storeA_compat_union_intro_l; assumption.
+           ++ rewrite <- map_union_assoc.
+              rewrite storeA_restrict_union_residual_l by exact Hcompat.
+              reflexivity.
+Qed.
+
 Lemma logic_qualifier_ext (q1 q2 : logic_qualifier) :
   lqual_dom q1 = lqual_dom q2 ->
   (forall (w1 : LWorldOnT (lqual_dom q1))
@@ -120,6 +207,68 @@ Proof.
   apply functional_extensionality. intros w.
   apply propositional_extensionality.
   apply HP. reflexivity.
+Qed.
+
+Lemma lqual_mlsubst_union
+    (ρ1 ρ2 : LStoreT) (q : logic_qualifier) :
+  storeA_compat ρ1 ρ2 ->
+  lqual_mlsubst ρ2 (lqual_mlsubst ρ1 q) =
+  lqual_mlsubst (ρ1 ∪ ρ2) q.
+Proof.
+  intros Hcompat.
+  destruct q as [D P]. cbn [lqual_mlsubst lqual_dom lqual_prop].
+  eapply logic_qualifier_ext.
+  - change ((D ∖ dom (ρ1 : gmap logic_var V)) ∖
+      dom (ρ2 : gmap logic_var V) =
+      D ∖ dom (ρ1 ∪ ρ2 : gmap logic_var V)).
+    apply set_eq. intros v.
+    rewrite !elem_of_difference, dom_union_L, elem_of_union.
+    tauto.
+  - intros w1 w2 Hlw. cbn [lqual_prop lqual_dom] in *.
+    pose proof (lworld_on_mlsubst_back_union D ρ1 ρ2 w1 w2 Hcompat Hlw)
+      as Hback.
+    rewrite Hback. reflexivity.
+Qed.
+
+Lemma lqual_mlsubst_empty (q : logic_qualifier) :
+  lqual_mlsubst (∅ : LStoreT) q = q.
+Proof.
+  destruct q as [D P].
+  cbn [lqual_mlsubst].
+  apply logic_qualifier_ext.
+  - change (D ∖ (∅ : lvset) = D).
+    apply difference_empty_L.
+  - intros w1 w2 Hlw. cbn [lqual_prop lqual_dom] in *.
+    enough (lworld_on_mlsubst_back D (∅ : LStoreT) w1 = w2) as ->.
+    { reflexivity. }
+    apply lworld_on_ext.
+    unfold lworld_on_mlsubst_back.
+    cbn [lw].
+    transitivity (@lw V (D ∖ dom (∅ : LStoreT)) w1).
+    + apply wfworldA_ext. apply worldA_ext.
+      * simpl.
+        unfold storeA_restrict.
+        replace (map_restrict V (∅ : LStoreT) D) with (∅ : LStoreT)
+          by (symmetry; apply map_restrict_idemp;
+              rewrite dom_empty_L; apply empty_subseteq).
+        change (dom (∅ : LStoreT)) with (∅ : lvset).
+        apply set_eq. intros z.
+        rewrite elem_of_union, elem_of_empty. tauto.
+      * intros σ. simpl.
+        unfold storeA_restrict.
+        replace (map_restrict V (∅ : LStoreT) D) with (∅ : LStoreT)
+          by (symmetry; apply map_restrict_idemp;
+              rewrite dom_empty_L; apply empty_subseteq).
+        split.
+        -- intros (σ1 & σ2 & Hσ1 & -> & _ & ->).
+           replace (σ1 ∪ ∅) with σ1 by (symmetry; apply map_union_empty).
+           exact Hσ1.
+        -- intros Hσ.
+           exists σ, (∅ : LStoreT). repeat split; try exact Hσ; try reflexivity.
+           ++ exact (ResourceAlgebra.rawA_compat_unit_r
+                (@lw V _ w1 : LWorldT) σ (∅ : LStoreT) Hσ eq_refl).
+           ++ symmetry. apply map_union_empty.
+    + exact Hlw.
 Qed.
 
 Lemma lqual_open_commute_fresh i j x y q :
